Use list

src/var.lean
@@ -1,13 +1,12 @@
 -- any infinite set would work
 def var: Type := string
 
-inductive cx (t: Type): Type
-| nil: cx
-| cons: cx -> var -> t -> cx
+@[reducible]
+def cx (t: Type) := list (prod var t)
 
-inductive lookup (t: Type): cx t -> var -> t -> Prop
-| hd (Γ: cx t) (x: var) (out: t): lookup (cx.cons Γ x out) x out
+inductive lookup {t: Type}: cx t -> var -> t -> Prop
+| hd (Γ: cx t) (x: var) (out: t): lookup (list.cons (prod.mk x out) Γ) x out
 | tl (Γ: cx t) (x: var) (out: t) (y: var) (out_y: t):
     x ≠ y ->
     lookup Γ x out ->
-    lookup (cx.cons Γ y out_y) x out
+    lookup (list.cons (prod.mk y out_y) Γ) x out
